Write proof sketch of theorem we want.
We want to show that we know the exact state of memory that is left
by the loop.

We show that looprev also leaves the same state.

Hence, they both make exactly the same changes to memory.

src/coq/LoopReversalManualProof.v
@@ -1116,6 +1116,11 @@ Proof.
   euttnorm.
 Qed.
 
+
+(** TODO: create a function that shows what memory looks like on n iterations **)
+Fixpoint create_mem_effect_of_loop (n: nat) (m: M.memory): M.memory := m.
+
+
   
 (** *Full effects *)
 
@@ -1123,12 +1128,12 @@ Qed.
 
 (** tiered semantics is already paying off, I can look at what happens
 when I execute a function **)
-Lemma mem_effect_main_function_orig: forall (n: nat) (initmem: M.memory) eff
+Lemma mem_effect_main_function_orig: forall (n: nat) (initmem: M.memory) 
   (N_GT_1: (n > 1)%nat),
-  M.memEffect initmem (SST.execFunction []
+  Trace.mapM fst (M.memEffect initmem (SST.execFunction []
               (SST.ENV.add (Name "main") (DVALUE_Addr (M.size  (a:=Z) M.empty, 0))
                  (SST.ENV.empty dvalue)) (SST.env_of_assoc []) 
-              (mainCFG n) (Name "main")) ≡ eff.
+              (mainCFG n) (Name "main"))) ≡ Ret (create_mem_effect_of_loop n initmem).
 Proof.
   Opaque SST.step_sem_tiered.
   Opaque SST.execBBInstrs.
@@ -1161,53 +1166,8 @@ Proof.
   setoid_rewrite SST.force_exec_function_at_bb_id; eauto.
   simpl.
   rewrite M.memEffect_commutes_with_bind; eauto.
-  rewrite exec_bbLoop_from_bbLoop.
 Abort.
   
-
-                                              
-
-(** Show this spurious proof to experiment with unfolding our new
-definition of program semantics **)
-Lemma run_mcfg_with_memory_orig:
-  forall (n: nat),
-    run_mcfg_with_memory_tiered (program n) ≡ 
-                                Ret (DVALUE_I32  (Int32.repr 1%Z)).
-Proof.
-  intros.
-  unfold run_mcfg_with_memory_tiered.
-  unfold SST.init_state_tiered.
-  unfold SST.build_global_environment_tiered.
-  unfold SST.allocate_globals_tiered.
-  simpl.
-  euttnorm.
-
-  unfold SST.register_functions_tiered.
-  simpl.
-  euttnorm.
-
-  unfold SST.register_declaration_tiered.
-  simpl.
-  euttnorm.
-
-  M.forcemem.
-  euttnorm.
-  
-  unfold SST.initialize_globals_tiered. simpl.
-  euttnorm.
-
-  rewrite SST.force_step_sem_tiered.
-  simpl.
-  
-  (** Need the opacity to make sure that Coq does not "unfold" too much **)
-  Opaque SST.execBB.
-  Opaque SST.step_sem_tiered.
-  Opaque SST.execFunction.
-  Opaque Trace.bindM.
-
-  
-  simpl.
-Abort.
   
 (* Lemma I care about *)
 Theorem looprev_same_semantics:
